chore: cleanup ReservationMap

Iris/Iris/Algebra/ReservationMap.lean
@@ -15,40 +15,42 @@ namespace Iris
 
 open Iris Std PartialMap
 
--- The camera [ReservationMap A H] over a camera [A] extends [LawfulPartialMap H Pos]
--- with a notion of "reservation tokens" for a (potentially infinite) set
--- [E : CoPset] which represent the right to allocate a map entry at any position
--- [k ∈ E].  The key connectives are [ReservationMap.singleton k a] (the "points-to"
--- assertion of this map), which associates data [a : A] with a key [k : Pos],
--- and [ReservationMap.token E] (the reservation token), which says
--- that no data has been associated with the indices in the mask [E]. The important
--- properties of this camera are:
---
--- • The lemma [ReservationMap.token_union] enables one to split [ReservationMap.token]
---   w.r.t. disjoint union. That is, if we have [E1 ## E2], then we get
---   [ReservationMap.token (E1 ∪ E2) = ReservationMap.token E1 • ReservationMap.token E2].
--- • The lemma [ReservationMap.alloc] provides a frame preserving update to
---   associate data to a key: [ReservationMap.token E ~~> ReservationMap.data k a]
---   provided [k ∈ E] and [✓ a].
---
--- In the future, it could be interesting to generalize this map to arbitrary key
--- types instead of hard-coding [Pos].
+/-!
+The camera [ReservationMap A H] over a camera [A] extends [LawfulPartialMap H Pos]
+with a notion of "reservation tokens" for a (potentially infinite) set
+[E : CoPset] which represent the right to allocate a map entry at any position
+[k ∈ E]. The key connectives are [ReservationMap.singleton k a] (the "points-to"
+assertion of this map), which associates data [a : A] with a key [k : Pos],
+and [ReservationMap.token E] (the reservation token), which says
+that no data has been associated with the indices in the mask [E]. The important
+properties of this camera are:
+
+• The lemma [ReservationMap.token_union] enables one to split [ReservationMap.token]
+  w.r.t. disjoint union. That is, if we have [E1 ## E2], then we get
+  [ReservationMap.token (E1 ∪ E2) = ReservationMap.token E1 • ReservationMap.token E2].
+• The lemma [ReservationMap.alloc] provides a frame preserving update to
+  associate data to a key: [ReservationMap.token E ~~> ReservationMap.data k a]
+  provided [k ∈ E] and [✓ a].
+
+NOTE: The keys type is currently fixed to be [Pos], though should be generalized
+in the future.
+-/
 
 @[rocq_alias reservation_map]
 structure ReservationMap (A : Type) (H : Type → Type) where
   dataProj : H A
   tokenProj : DisjointLeibnizSet CoPset
 
-def ReservationMap.data [LawfulPartialMap H Pos] (data : H A)
-    : ReservationMap A H := .mk data ∅
+def ReservationMap.data [LawfulPartialMap H Pos] (data : H A) :
+    ReservationMap A H := .mk data ∅
 
 @[rocq_alias reservation_map_data]
-def ReservationMap.singleton [LawfulPartialMap H Pos] (k : Pos) (a : A)
-    : ReservationMap A H := ReservationMap.data {[k := a]}
+def ReservationMap.singleton [LawfulPartialMap H Pos] (k : Pos) (a : A) :
+    ReservationMap A H := ReservationMap.data {[k := a]}
 
 @[rocq_alias reservation_map_token]
-def ReservationMap.token [LawfulPartialMap H Pos] (e : CoPset)
-    : ReservationMap A H := .mk ∅ (.valid e)
+def ReservationMap.token [LawfulPartialMap H Pos] (e : CoPset) :
+    ReservationMap A H := .mk ∅ (.valid e)
 
 section OFE
 
@@ -63,37 +65,43 @@ instance : OFE (ReservationMap A H) where
   Equiv x y := x.dataProj ≡ y.dataProj ∧ x.tokenProj ≡ y.tokenProj
   Dist n x y := x.dataProj ≡{n}≡ y.dataProj ∧ x.tokenProj ≡{n}≡ y.tokenProj
   dist_eqv := {
-    refl _ := ⟨OFE.Dist.rfl, rfl⟩,
-    symm h := ⟨Dist.symm h.left, Eq.symm h.right⟩,
-    trans h₁ h₂ := ⟨Dist.trans h₁.left h₂.left, Eq.trans h₁.right h₂.right⟩
+    refl _ := ⟨.rfl, rfl⟩,
+    symm h := ⟨h.left.symm, h.right.symm⟩,
+    trans h₁ h₂ := ⟨h₁.left.trans h₂.left, h₁.right.trans h₂.right⟩
   }
-  equiv_dist := ⟨fun h n => ⟨equiv_dist.mp h.left n, h.right⟩
-               , fun h => ⟨equiv_dist.mpr (fun n => (h n).left), (h 0).right⟩⟩
+  equiv_dist :=
+    ⟨fun h n => ⟨equiv_dist.mp h.left n, h.right⟩,
+     fun h => ⟨equiv_dist.mpr (h · |>.left), (h 0).right⟩⟩
   dist_lt h lt := ⟨dist_lt h.left lt, dist_lt h.right lt⟩
 
 @[rocq_alias reservation_map_ofe_discrete]
-instance [Discrete A] : Discrete (ReservationMap A H) where
+instance instDiscreteReservationMap [Discrete A] : Discrete (ReservationMap A H) where
   discrete_0 h := ⟨discrete_0 h.left, discrete_0 h.right⟩
 
-instance : NonExpansive (ReservationMap.data (H := H) (A := A)) where
+instance instNonExpansiveReservationMapData :
+    NonExpansive (ReservationMap.data (H := H) (A := A)) where
   ne _ _ _ h := ⟨h, Dist.rfl⟩
 
 #rocq_ignore reservation_map_data_proper "Derivable using NonExpansive.eqv"
 
 @[rocq_alias reservation_map_data_ne]
-instance : NonExpansive (ReservationMap.singleton (H := H) (A := A) k) where
+instance instNonExpansiveReservationMapSingleton :
+    NonExpansive (ReservationMap.singleton (H := H) (A := A) k) where
   ne _ _ _ h := ⟨singleton_dist h k, Dist.rfl⟩
 
 @[rocq_alias ReservationMap_discrete]
-instance {a : H A} [DiscreteE a] : DiscreteE (ReservationMap.mk a b) where
+instance instDiscreteEReservationMapMk {a : H A} [DiscreteE a] :
+    DiscreteE (ReservationMap.mk a b) where
   discrete := fun ⟨ha, hb⟩ => ⟨DiscreteE.discrete ha, DiscreteE.discrete hb⟩
 
 @[rocq_alias reservation_map_data_discrete]
-instance {a : A} [DiscreteE a] : DiscreteE (ReservationMap.singleton (H := H) k a) :=
+instance instDiscreteEReservationMapSingleton {a : A} [DiscreteE a] :
+    DiscreteE (ReservationMap.singleton (H := H) k a) :=
   by unfold ReservationMap.singleton ReservationMap.data;  infer_instance
 
 @[rocq_alias reservation_map_token_discrete]
-instance : DiscreteE (ReservationMap.token (H := H) (A := A) e) :=
+instance instDiscreteEReservationMapToken :
+    DiscreteE (ReservationMap.token (H := H) (A := A) e) :=
   by unfold ReservationMap.token; infer_instance
 
 end OFE
@@ -116,75 +124,73 @@ def Valid (x : ReservationMap A H) : Prop :=
   | .valid e => ✓ x.dataProj ∧ ∀i, get? x.dataProj i = none ∨ i ∉ e
   | .error => False
 
-def validN_unpack {n : Nat} {x : ReservationMap A H} (h : x.ValidN n)
-    : ✓{n} x.dataProj ∧ ✓{n} x.tokenProj ∧ ∀i, get? x.dataProj i = none ∨ i ∉ x.tokenProj := by
+def validN_unpack {n : Nat} {x : ReservationMap A H} (h : x.ValidN n) :
+    ✓{n} x.dataProj ∧ ✓{n} x.tokenProj ∧ ∀i, get? x.dataProj i = none ∨ i ∉ x.tokenProj := by
   simp only [ValidN] at h
-  match eq : x.tokenProj with
-  | .valid s =>
-    exact ⟨(eq ▸ h).left, (valid_0_iff_validN n).mp trivial, (eq ▸ h).right⟩
-  | .error => exact (eq ▸ h).elim
+  exact match eq : x.tokenProj with
+  | .valid s => ⟨(eq ▸ h).left, (valid_0_iff_validN n).mp trivial, (eq ▸ h).right⟩
+  | .error => (eq ▸ h).elim
 
-theorem validN_dataProj_of_validN {n : Nat} {x : ReservationMap A H} (h : x.ValidN n)
-    : ✓{n} x.dataProj := (validN_unpack h).left
+theorem validN_dataProj_of_validN {n : Nat} {x : ReservationMap A H} (h : x.ValidN n) :
+    ✓{n} x.dataProj := (validN_unpack h).left
 
-theorem validN_tokenProj_of_validN {n : Nat} {x : ReservationMap A H} (h : x.ValidN n)
-    : ✓{n} x.tokenProj := (validN_unpack h).right.left
+theorem validN_tokenProj_of_validN {n : Nat} {x : ReservationMap A H} (h : x.ValidN n) :
+    ✓{n} x.tokenProj := (validN_unpack h).right.left
 
-theorem validN_disj {n : Nat} {x : ReservationMap A H} (h : x.ValidN n)
-    : ∀i, get? x.dataProj i = none ∨ i ∉ x.tokenProj := (validN_unpack h).right.right
+theorem validN_disj {n : Nat} {x : ReservationMap A H} (h : x.ValidN n) (i : Pos) :
+  get? x.dataProj i = none ∨ i ∉ x.tokenProj := (validN_unpack h).right.right i
 
-theorem validN_of_parts {n : Nat} {x : ReservationMap A H}
-    (vd : ✓{n} x.dataProj) (vt : ✓{n} x.tokenProj)
-    (disj : ∀i, get? x.dataProj i = none ∨ i ∉ x.tokenProj)
-    : x.ValidN n := by
+theorem validN_of_parts {n : Nat} {x : ReservationMap A H} (vd : ✓{n} x.dataProj)
+    (vt : ✓{n} x.tokenProj) (disj : ∀i, get? x.dataProj i = none ∨ i ∉ x.tokenProj) :
+    x.ValidN n := by
   simp only [ValidN]
   cases h : x.tokenProj
   · simp only [h] at disj
     exact ⟨vd, disj⟩
   · exact ((h ▸ not_valid_invalid (S := CoPset)) vt)
 
-def valid_unpack {x : ReservationMap A H} (h : x.Valid)
-    : ✓ x.dataProj ∧ ✓ x.tokenProj ∧ ∀i, get? x.dataProj i = none ∨ i ∉ x.tokenProj := by
+def valid_unpack {x : ReservationMap A H} (h : x.Valid) :
+    ✓ x.dataProj ∧ ✓ x.tokenProj ∧ ∀i, get? x.dataProj i = none ∨ i ∉ x.tokenProj := by
   simp only [Valid] at h
-  match eq : x.tokenProj with
-  | .valid s =>
-    exact ⟨(eq ▸ h).left, valid_mapN (fun n a => a) trivial, (eq ▸ h).right⟩
-  | .error => exact (eq ▸ h).elim
+  exact match eq : x.tokenProj with
+  | .valid s => ⟨(eq ▸ h).left, valid_mapN (fun n a => a) trivial, (eq ▸ h).right⟩
+  | .error => (eq ▸ h).elim
 
-theorem valid_dataProj_of_valid {x : ReservationMap A H} (h : x.Valid)
-    : ✓ x.dataProj := (valid_unpack h).left
+theorem valid_dataProj_of_valid {x : ReservationMap A H} (h : x.Valid) :
+    ✓ x.dataProj := (valid_unpack h).left
 
-theorem valid_tokenProj_of_valid {x : ReservationMap A H} (h : x.Valid)
-    : ✓ x.tokenProj := (valid_unpack h).right.left
+theorem valid_tokenProj_of_valid {x : ReservationMap A H} (h : x.Valid) :
+    ✓ x.tokenProj := (valid_unpack h).right.left
 
-theorem valid_disj {x : ReservationMap A H} (h : x.Valid)
-    : ∀i, get? x.dataProj i = none ∨ i ∉ x.tokenProj := (valid_unpack h).right.right
+theorem valid_disj {x : ReservationMap A H} (h : x.Valid) (i : Pos):
+    get? x.dataProj i = none ∨ i ∉ x.tokenProj := (valid_unpack h).right.right i
 
-theorem valid_of_parts {x : ReservationMap A H}
-    (vd : ✓ x.dataProj) (vt : ✓ x.tokenProj)
-    (disj : ∀i, get? x.dataProj i = none ∨ i ∉ x.tokenProj)
-    : x.Valid := by
+theorem valid_of_parts {x : ReservationMap A H} (vd : ✓ x.dataProj) (vt : ✓ x.tokenProj)
+    (disj : ∀i, get? x.dataProj i = none ∨ i ∉ x.tokenProj) : x.Valid := by
   simp only [Valid]
   cases h : x.tokenProj
   · simp only [h] at disj
     exact ⟨vd, disj⟩
   · exact (h ▸ not_valid_invalid) vt
 
-def core (x : ReservationMap A H) : ReservationMap A H :=
-  mk (CMRA.core x.dataProj) ∅
+def core (x : ReservationMap A H) : ReservationMap A H := mk (CMRA.core x.dataProj) ∅
 
-theorem core_dataProj (x : ReservationMap A H) : x.core.dataProj = CMRA.core x.dataProj :=
-  rfl
+@[simp]
+theorem core_dataProj (x : ReservationMap A H) :
+  x.core.dataProj = CMRA.core x.dataProj := rfl
 
+@[simp]
 theorem core_tokenProj (x : ReservationMap A H) : x.core.tokenProj = CMRA.core x.tokenProj :=
   rfl
 
 def op (x y : ReservationMap A H) : ReservationMap A H :=
   mk (x.dataProj • y.dataProj) (x.tokenProj • y.tokenProj)
 
+@[simp]
 theorem op_dataProj' (x y : ReservationMap A H): (x.op y).dataProj = x.dataProj • y.dataProj :=
   rfl
 
+@[simp]
 theorem op_tokenProj' (x y : ReservationMap A H): (x.op y).tokenProj = x.tokenProj • y.tokenProj :=
   rfl
 
@@ -246,9 +252,9 @@ instance : UCMRA (ReservationMap A H) where
         simp only [op_dataProj', Heap.get?_op] at aa
         exact .inl <| Option.eq_none_of_op_eq_none_left aa
       | inr bb =>
-        exact .inr <| bb
-          ∘ (mem_iff_of_validN_union (validN_tokenProj_of_validN v) i).mpr
-          ∘ .inl
+        refine .inr fun HK => bb ?_
+        refine (mem_iff_of_validN_union (validN_tokenProj_of_validN v) i).mpr ?_
+        exact .inl HK
   assoc := ⟨CMRA.assoc, CMRA.assoc⟩
   comm := ⟨CMRA.comm, CMRA.comm⟩
   pcore_op_left {x cx} h := by
@@ -269,7 +275,7 @@ instance : UCMRA (ReservationMap A H) where
   extend {n x y₁ y₂} v exy := by
     obtain ⟨z₁, z₂, xzz, zy₁, zy₂⟩ := CMRA.extend (validN_dataProj_of_validN v) exy.left
     refine ⟨mk z₁ y₁.tokenProj, mk z₂ y₂.tokenProj, ?_, ?_, ?_⟩
-    · exact ⟨by simp [op_dataProj', xzz], by simp [op_tokenProj'];  exact exy.right⟩
+    · exact ⟨by simp [op_dataProj', xzz], by simpa [op_tokenProj'] using exy.right⟩
     · exact ⟨zy₁, rfl⟩
     · exact ⟨zy₂, rfl⟩
   unit := mk ∅ ∅
@@ -277,9 +283,11 @@ instance : UCMRA (ReservationMap A H) where
   unit_left_id {x} := ⟨by simp only [op, Algebra.MonoidOps.op_left_id], pcore_op_left' rfl⟩
   pcore_unit := ⟨Heap.core_empty, .rfl⟩
 
+@[simp]
 theorem op_dataProj (x y : ReservationMap A H): (x • y).dataProj = x.dataProj • y.dataProj :=
   rfl
 
+@[simp]
 theorem op_tokenProj (x y : ReservationMap A H): (x • y).tokenProj = x.tokenProj • y.tokenProj :=
   rfl
 
@@ -289,13 +297,13 @@ instance [CMRA.Discrete A] : CMRA.Discrete (ReservationMap A H) where
     valid_of_parts (discrete_valid (validN_dataProj_of_validN v))
       (validN_tokenProj_of_validN v) (validN_disj v)
 
-instance {a : A} [CoreId a] : CoreId (singleton (H := H) k a) where
-  core_id :=
-    ⟨ by simp [core_dataProj, singleton, data, core_eqv_self (PartialMap.singleton k a)]
-    , rfl ⟩
+instance instCoreIdSingleton {a : A} [CoreId a] : CoreId (singleton (H := H) k a) where
+  core_id := by
+    refine ⟨?_, rfl⟩
+    simp [singleton, data, core_eqv_self (PartialMap.singleton k a)]
 
-theorem split_valid {x : ReservationMap A H} (vx : ✓ x)
-    : ∃(d : H A) (t : _), x ≡ data d • token t := by
+theorem split_valid {x : ReservationMap A H} (vx : ✓ x) :
+    ∃ (d : H A) (t : CoPset), x ≡ data d • token t := by
   rcases x with ⟨xd, xt⟩
   match hh : xt with
   | .error =>
@@ -306,35 +314,28 @@ theorem split_valid {x : ReservationMap A H} (vx : ✓ x)
     . simp only [data, token, op_tokenProj, leibniz]
       exact (pcore_op_left_L rfl).symm
 
-theorem split_validN {x : ReservationMap A H} (vx : ✓{n} x)
-    : ∃(d : H A) (t : _), x ≡ data d • token t := by
+theorem split_validN {x : ReservationMap A H} (vx : ✓{n} x) :
+    ∃ (d : H A) (t : CoPset), x ≡ data d • token t := by
   rcases x with ⟨xd, xt⟩
-  have := validN_tokenProj_of_validN vx
+  have H := validN_tokenProj_of_validN vx
   match hh : xt with
-  | .error => exact ((not_valid_invalid (S := CoPset)) (hh ▸ this)).elim
+  | .error => exact ((not_valid_invalid (S := CoPset)) (hh ▸ H)).elim
   | .valid t =>
     refine ⟨xd, t, ?_, ?_⟩
-    · simp only [data, token, op_dataProj]
-      exact Algebra.MonoidOps.op_right_id.symm
+    · simpa [data, token, op_dataProj] using Algebra.MonoidOps.op_right_id.symm
     . exact (pcore_op_left' rfl).symm
 
-theorem valid_data {d : H A}
-    : ✓ (data (H := H) d) ↔ ✓ d :=
-  ⟨ valid_dataProj_of_valid
-  , fun h => valid_of_parts h ⟨⟩ (fun p => .inr (mem_empty p))⟩
+theorem valid_data {d : H A} : ✓ (data (H := H) d) ↔ ✓ d :=
+  ⟨valid_dataProj_of_valid, fun h => valid_of_parts h ⟨⟩ (fun p => .inr (mem_empty p))⟩
 
-theorem validN_data {d : H A}
-    : ✓{n} (data (H := H) d) ↔ ✓{n} d :=
-  ⟨ validN_dataProj_of_validN
-  , fun h => validN_of_parts h ⟨⟩ (fun p => .inr (mem_empty p))⟩
+theorem validN_data {d : H A} : ✓{n} (data (H := H) d) ↔ ✓{n} d :=
+  ⟨validN_dataProj_of_validN, fun h => validN_of_parts h ⟨⟩ (fun p => .inr (mem_empty p))⟩
 
 @[rocq_alias reservation_map_data_valid]
-theorem valid_singleton (k : Pos) (a : A)
-    : ✓ (singleton (H := H) k a) ↔ ✓ a :=
+theorem valid_singleton (k : Pos) (a : A) : ✓ (singleton (H := H) k a) ↔ ✓ a :=
   (valid_data).trans Heap.singleton_valid_iff
 
-theorem validN_singleton (k : Pos) (a : A)
-    : ✓{n} (singleton (H := H) k a) ↔ ✓{n} a :=
+theorem validN_singleton (k : Pos) (a : A) : ✓{n} (singleton (H := H) k a) ↔ ✓{n} a :=
   (validN_data).trans Heap.singleton_validN_iff
 
 @[rocq_alias reservation_map_token_valid]
@@ -344,22 +345,19 @@ theorem valid_token : ✓ (token (H := H) (A := A) e) :=
 theorem data_op (a b : H A) : data (a • b) ≡ data a • data b :=
   ⟨.rfl, (pcore_op_right_L rfl).symm⟩
 
-open Classical in
 @[rocq_alias reservation_map_data_op]
-theorem singleton_op k (a b : A)
-    : singleton (H := H) k (a • b) ≡ singleton (H := H) k a • singleton k b := by
+theorem singleton_op k (a b : A) :
+    singleton (H := H) k (a • b) ≡ singleton (H := H) k a • singleton k b := by
   refine ((data_op _ _).symm.trans ?_).symm
   exact NonExpansive.eqv (fun i => .of_eq (Heap.singleton_op_singleton i))
 
-theorem token_op (a b : CoPset) (h : a ## b)
-    : token (H := H) (A := A) (a ∪ b) ≡ token a • token b := by
+theorem token_op (a b : CoPset) (h : a ## b) :
+    token (H := H) (A := A) (a ∪ b) ≡ token a • token b := by
   refine ⟨show ∅ ≡ (∅ : H A) • ∅ from Algebra.MonoidOps.op_left_id.symm, ?_⟩
   simp [token, CMRA.op, op_tokenProj', h]
 
-theorem disj_of_validN_data_op_token {a : H A} {b : CoPset}
-    (h : ✓{n} data a • token b)
-    : ∀i, get? a i = none ∨ i ∉ b := by
-  intro i
+theorem disj_of_validN_data_op_token {a : H A} {b : CoPset} (h : ✓{n} data a • token b) (i : Pos) :
+    get? a i = none ∨ i ∉ b := by
   cases validN_disj h i with
   | inl h =>
     simp only [data, token, op_dataProj, Heap.get?_op, get?_empty] at h
@@ -370,104 +368,80 @@ theorem disj_of_validN_data_op_token {a : H A} {b : CoPset}
     · exact .inr <| fun hh => h'.right hh
     · exact valid_of_eqv (pcore_op_left' rfl).symm valid_set
 
-theorem disj_of_valid_data_op_token (a : H A) (b : CoPset)
-    (h : ✓ data a • token b)
-    : ∀i, get? a i = none ∨ i ∉ b := disj_of_validN_data_op_token (h.validN (n := 0))
+theorem disj_of_valid_data_op_token (a : H A) (b : CoPset) (h : ✓ data a • token b) (i : Pos) :
+  get? a i = none ∨ i ∉ b := disj_of_validN_data_op_token (h.validN (n := 0)) i
 
-theorem validN_data_op_token {n : Nat} (a : H A) (b : CoPset)
-    (vd : ✓{n} data a) (disj : ∀i, get? a i = none ∨ i ∉ b)
-    : ✓{n} data a • token b := by
+theorem validN_data_op_token {n : Nat} (a : H A) (b : CoPset) (vd : ✓{n} data a)
+    (disj : ∀ i, get? a i = none ∨ i ∉ b) : ✓{n} data a • token b := by
   have abdp : (data a • token b).dataProj ≡ a :=
     show a • ∅ ≡ a from (Algebra.MonoidOps.op_right_id)
   have eo : ∅ • valid b = .valid b := pcore_op_left_L rfl
-  refine validN_of_parts
-    (validN_of_eqv abdp.symm ((validN_data).mp vd))
+  refine validN_of_parts (validN_of_eqv abdp.symm ((validN_data).mp vd))
     (by simp [op_tokenProj, data, token, eo, validN_set])
-    ?_
-  · intro i
-    simp only [data, token, op_dataProj, Heap.get?_op, get?_empty, op_tokenProj]
-    cases disj i with
-    | inl h =>
-      simp only [h]
-      exact .inl <| rfl
-    | inr h =>
-      simp only [eo]
-      exact .inr h
+    fun i => ?_
+  simp only [data, token, op_dataProj, Heap.get?_op, get?_empty, op_tokenProj]
+  cases disj i with
+  | inl h => simpa [h] using .inl <| rfl
+  | inr h => simpa [eo] using .inr h
 
-theorem valid_data_op_token (a : H A) (b : CoPset)
-    (vd : ✓ data a) (disj : ∀i, get? a i = none ∨ i ∉ b)
-    : ✓ data a • token b := by
+theorem valid_data_op_token (a : H A) (b : CoPset) (vd : ✓ data a)
+    (disj : ∀i, get? a i = none ∨ i ∉ b) : ✓ data a • token b := by
   have abdp : (data a • token b).dataProj ≡ a :=
     show a • ∅ ≡ a from (Algebra.MonoidOps.op_right_id)
   have eo : ∅ • valid b = .valid b := pcore_op_left_L rfl
-  refine valid_of_parts
-    (valid_of_eqv abdp.symm ((valid_data).mp vd))
+  refine valid_of_parts (valid_of_eqv abdp.symm ((valid_data).mp vd))
     (by simp [op_tokenProj, data, token, eo, valid_set])
-    ?_
-  · intro i
-    simp only [data, token, op_dataProj, Heap.get?_op, get?_empty, op_tokenProj]
-    cases disj i with
-    | inl h =>
-      simp only [h]
-      exact .inl <| rfl
-    | inr h =>
-      simp only [eo]
-      exact .inr h
+    fun i => ?_
+  simp only [data, token, op_dataProj, Heap.get?_op, get?_empty, op_tokenProj]
+  cases disj i with
+  | inl h => simpa only [h] using .inl <| rfl
+  | inr h => simpa only [eo] using .inr h
 
 @[rocq_alias reservation_map_data_mono]
-theorem singleton_mono k (a b : A)
-    : a ≼ b → singleton (H := H) k a ≼ singleton k b :=
-  fun ⟨z, hz⟩ => ⟨singleton k z, (NonExpansive.eqv hz).trans (singleton_op k a z)⟩
+theorem singleton_mono {k} {a b : A} (Hab : a ≼ b) : singleton (H := H) k a ≼ singleton k b :=
+  let ⟨z, hz⟩ := Hab
+  ⟨singleton k z, (NonExpansive.eqv hz).trans (singleton_op k a z)⟩
 
 set_option synthInstance.checkSynthOrder false in
 @[rocq_alias reservation_map_data_is_op]
-instance {ia ib₁ ib₂ : ProofMode.InOut} {a b₁ b₂ : A} [hv : IsOp ia a ib₁ b₁ ib₂ b₂]
-  : IsOp ia (singleton (H := H) k a) ib₁ (singleton k b₁) ib₂ (singleton k b₂) where
+instance {ia ib₁ ib₂ : ProofMode.InOut} {a b₁ b₂ : A} [hv : IsOp ia a ib₁ b₁ ib₂ b₂] :
+    IsOp ia (singleton (H := H) k a) ib₁ (singleton k b₁) ib₂ (singleton k b₂) where
   is_op := .trans (NonExpansive.eqv hv.is_op ) (singleton_op k b₁ b₂)
 
 @[rocq_alias reservation_map_token_union]
-theorem token_union {e₁ e₂} (he : e₁ ## e₂)
-    : token (H := H) (A := A) (e₁ ∪ e₂) ≡
-      token e₁ • token e₂ := by
+theorem token_union {e₁ e₂} (he : e₁ ## e₂) :
+    token (H := H) (A := A) (e₁ ∪ e₂) ≡ token e₁ • token e₂ := by
   refine ⟨fun i => ?_, ?_⟩
-  · simp only [token, get?_empty, op_dataProj, Heap.get?_op]
-    exact .rfl
-  · simp only [token, op_tokenProj, leibniz]
-    simp [CMRA.op, he]
+  · simpa only [token, get?_empty, op_dataProj, Heap.get?_op] using .rfl
+  · simp [token, CMRA.op, he]
 
 @[rocq_alias reservation_map_token_difference]
-theorem token_difference {e₁ e₂} (he : e₁ ⊆ e₂)
-    : token (H := H) (A := A) e₂ ≡
-      token e₁ • token (e₂ \ e₁) := by
+theorem token_difference {e₁ e₂} (he : e₁ ⊆ e₂) :
+    token (H := H) (A := A) e₂ ≡ token e₁ • token (e₂ \ e₁) := by
   refine .trans ?_ (token_union LawfulSet.disjoint_diff_right)
   rw [LawfulSet.subset_union_diff he]
 
 @[rocq_alias reservation_map_token_valid_op]
-theorem valid_token_op_iff_disj {e₁ e₂}
-    : ✓ (token (H := H) (A := A) e₁ • token e₂) ↔ e₁ ## e₂ :=
-  ⟨ fun h => valid_op_iff_disj.mp (valid_tokenProj_of_valid h)
-  , fun h => (Equiv.valid (token_union h)).mp valid_token⟩
+theorem valid_token_op_iff_disj {e₁ e₂} :
+    ✓ (token (H := H) (A := A) e₁ • token e₂) ↔ e₁ ## e₂ :=
+  ⟨fun h => valid_op_iff_disj.mp (valid_tokenProj_of_valid h),
+   fun h => (Equiv.valid (token_union h)).mp valid_token⟩
 
-theorem validN_token_op_iff_disj {e₁ e₂}
-    : ✓{n} (token (H := H) (A := A) e₁ • token e₂) ↔ e₁ ## e₂ where
+theorem validN_token_op_iff_disj {e₁ e₂} :
+    ✓{n} (token (H := H) (A := A) e₁ • token e₂) ↔ e₁ ## e₂ where
   mp h := valid_op_iff_disj.mp (validN_tokenProj_of_validN h)
   mpr h := by
-    refine validN_of_parts ?_ ?_ ?_
+    refine validN_of_parts ?_ ?_ fun i => ?_
     · show ✓{n} ∅ • (∅ : H A)
       refine validN_of_eqv Algebra.MonoidOps.op_left_id.symm ?_
       exact Heap.valid_empty.validN
-    · simp only [CMRA.op, token, op, h]
-      exact validN_set
-    · intro i
-      simp [token, op_dataProj, op_tokenProj, Heap.get?_op, get?_empty]
-      exact .inl rfl
+    · simpa [CMRA.op, token, op, h] using validN_set
+    · simpa [token, op_dataProj, op_tokenProj, Heap.get?_op, get?_empty] using .inl rfl
 
-theorem valid_op?_of_valid_singleton_op {a : A} {x : H A} (h : ✓{n} (singleton k a • data x))
-    : ✓{n} a •? get? x k := by
+theorem valid_op?_of_valid_singleton_op {a : A} {x : H A} (h : ✓{n} (singleton k a • data x)) :
+    ✓{n} a •? get? x k := by
   match h' : get? x k with
-  | none =>
-    simp only [op?]
-    exact (validN_singleton (H := H) k a).mp (validN_op_left h)
+  | none => simpa [op?] using (validN_singleton (H := H) k a).mp (validN_op_left h)
   | some g =>
     simp only [op?]
     have vdp := (validN_dataProj_of_validN h) k
@@ -475,46 +449,42 @@ theorem valid_op?_of_valid_singleton_op {a : A} {x : H A} (h : ✓{n} (singleton
       LawfulPartialMap.get?_singleton, ↓reduceIte, h'] at vdp
     exact vdp
 
-theorem valid_singleton_op_of_valid_op? {a : A} {x : H A} (vx : ✓{n} x) (h : ✓{n} a •? get? x k)
-    : ✓{n} singleton k a • data x := by
+theorem valid_singleton_op_of_valid_op? {a : A} {x : H A} (vx : ✓{n} x) (h : ✓{n} a •? get? x k) :
+    ✓{n} singleton k a • data x := by
   refine validN_of_eqv (data_op (PartialMap.singleton k a) x) ?_
-  refine (validN_data).mpr ?_
-  intro i
+  refine (validN_data).mpr fun i => ?_
   rw [Heap.get?_op]
   by_cases ki : k = i
-  · simp only [← ki, LawfulPartialMap.get?_singleton, ↓reduceIte, Option.some_op_opM]
-    exact h
-  · simp only [LawfulPartialMap.get?_singleton, ki, ↓reduceIte]
-    exact Heap.validN_get? vx
+  · simpa only [← ki, LawfulPartialMap.get?_singleton, ↓reduceIte, Option.some_op_opM] using h
+  · simpa only [LawfulPartialMap.get?_singleton, ki, ↓reduceIte] using Heap.validN_get? vx
 
 @[rocq_alias reservation_map_alloc]
-theorem alloc {e k} {a : A} (hke : k ∈ e) (va : ✓ a)
-    : token (H := H) e ~~> singleton k a := by
+theorem alloc {e k} {a : A} (hke : k ∈ e) (va : ✓ a) : token (H := H) e ~~> singleton k a := by
   intro n mz vo
   match mz with
   | none => exact Valid.validN <| (valid_singleton k a).mpr va
   | some z =>
     have ⟨d, t, ze⟩ := split_validN (validN_op_right vo)
     have vedt : ✓{n} token e • (data d • token t) := validN_of_eqv (op_right_eqv _ ze) vo
-    have disj := disj_of_validN_data_op_token (validN_of_eqv CMRA.comm (validN_op_left (validN_of_eqv CMRA.assoc vedt)))
+    have disj : ∀ (i : Pos), get? d i = none ∨ ¬i ∈ e:=
+      disj_of_validN_data_op_token (validN_of_eqv comm (validN_op_left (validN_of_eqv assoc vedt)))
     refine validN_of_eqv (op_right_eqv _ ze.symm) ?_
     refine validN_of_eqv CMRA.assoc.symm ?_
     refine validN_of_eqv (op_left_eqv (token t) (data_op _ _)) ?_
     refine validN_data_op_token (PartialMap.singleton k a • d) t ?_ ?_
     · refine validN_of_eqv (data_op _ _).symm ?_
       apply valid_singleton_op_of_valid_op?
-      · exact validN_data.mp (validN_op_left (validN_of_eqv CMRA.comm (validN_op_left (validN_of_eqv CMRA.assoc vedt))))
+      · exact validN_data.mp (validN_op_left (validN_of_eqv comm (validN_op_left (validN_of_eqv assoc vedt))))
       · exact (disj k).elim (fun h => h ▸ Valid.validN va) (absurd hke)
     · simp only [CMRA.op, Heap.op, get?_merge, LawfulPartialMap.get?_singleton,
         Option.merge_eq_none_iff, ite_eq_right_iff, reduceCtorEq, imp_false]
       intro i
-      grind [disj_of_validN_data_op_token (validN_of_eqv ze (validN_op_right vo))
-        , validN_token_op_iff_disj.mp (validN_op_right (validN_of_eqv CMRA.assoc.symm (validN_of_eqv CMRA.comm vedt))) i]
+      grind [disj_of_validN_data_op_token (validN_of_eqv ze (validN_op_right vo)),
+        validN_token_op_iff_disj.mp (validN_op_right (validN_of_eqv assoc.symm (validN_of_eqv comm vedt))) i]
 
 @[rocq_alias reservation_map_updateP]
-theorem updateP {P} {Q : ReservationMap A H → Prop} k a
-    (ap : a ~~>: P) (apq : ∀ a', P a' → Q (singleton k a')) :
-    singleton k a ~~>: Q := by
+theorem updateP {P} {Q : ReservationMap A H → Prop} k a (ap : a ~~>: P)
+    (apq : ∀ a', P a' → Q (singleton k a')) : singleton k a ~~>: Q := by
   intro n mz vaz
   match mz with
   | none =>
@@ -545,7 +515,7 @@ theorem updateP {P} {Q : ReservationMap A H → Prop} k a
       grind
 
 @[rocq_alias reservation_map_update]
-theorem reservation_map_update k (a b : A) (uab : a ~~> b):
+theorem reservation_map_update {k} {a b : A} (uab : a ~~> b):
     singleton (H := H) k a ~~> singleton k b :=
   Update.of_updateP <| updateP k a (.of_update uab) fun _ => congrArg (singleton k)
 
